AP/AP/Defense/Edge/Symmetry.lean
@@ -1,4 +1,3 @@
 import AP.AP.Defense.Edge.Symmetry.Basic
 import AP.AP.Defense.Edge.Symmetry.Translation
 import AP.AP.Defense.Edge.Symmetry.Rotation
-import AP.AP.Defense.Edge.Symmetry.Reflection
